an experiment for better tactics, stalled until coqfixes some strange behaviour (coq PR #8357)

LibDecomp.v
@@ -5,7 +5,7 @@ Ltac decomp_logicals h :=
   | @ex _ (fun x => _) => let x' := fresh x in let h1 := fresh in destruct h as [x' h1]; decomp_logicals h1
   | @sig _ (fun x => _) => let x' := fresh x in let h1 := fresh in destruct h as [x' h1]; decomp_logicals h1
   | @sig2 _ (fun x => _) (fun _ => _) => let x' := fresh x in
-                                         let h1 := fresh in 
+                                         let h1 := fresh in
                                          let h2 := fresh in
                                          destruct h as [x' h1 h2];
                                          decomp_logicals h1;
@@ -23,20 +23,60 @@ Ltac decomp_logicals h :=
 (*
 Lemma foo : forall x, { aa:nat | (aa = x /\ x=aa) & (aa = aa /\ aa= x) } -> False.
 Proof.
-  intros x h. 
+  intros x h.
   pose proof h as h'.
 Abort.
 
 Lemma foo : { aa:False & True  } -> False.
 Proof.
-  intros H. 
+  intros H.
   decomp H.
 Abort.
 
 
 Lemma foo : { aa:False & True & False  } -> False.
 Proof.
-  intros H. 
+  intros H.
   decomp H.
 Abort.
+*)
+
+(* proveprem H at i as h. Create an assert for the ith dependent
+premiss of hypothesis H and specialize H with the resulting proof. h
+is the (optional) name of the asserted premiss. *)
+
+Ltac proveprem_ H i id :=
+  (* prefer this to evar, which is not well "typed" by Ltac (does not
+  know that it creates an evar (coq bug?). *)
+  let ev := open_constr:((_:Prop)) in
+  assert (id:ev);
+  [|specialize H with (i:=id)].
+
+Tactic Notation "proveprem" hyp(H) "at" integer(i) "as" ident(id)  :=
+  proveprem_ H i id.
+
+Tactic Notation "proveprem" hyp(H) "at" integer(i) :=
+  let id := fresh H "_prem" in
+  proveprem_ H i id.
+
+(*
+Definition test n := n = 1.
+Variable Q: nat -> bool -> list nat -> Prop.
+Lemma foo:
+  (forall n b l, b = true -> test n -> Q n b l) ->
+  (true = true -> false = false ->  True) -> Q 1 true (cons 1 nil).
+Proof.
+  intros hyp hyp'.
+  (* proveprem hyp at 2 as h. *)
+  let ev := open_constr:((_:Prop)) in
+  assert (id:ev).
+  2:specialize hyp with (2:=id).
+  { reflexivity. }
+  Check h.
+  proveprem hyp at 1.
+  { reflexivity. }
+  Check hyp_prem.
+  apply hyp.
+Qed.
+
 *)
