TemporaryNotations.v
@@ -1,3 +1,5 @@
+Require Import sparkfrontend.compcert_utils  compcert.backend.Cminor compcert.lib.Integers.
+
 Notation "[ '**' '|_|' N '+' X ]" := (build_loads_ X N) (at level 0).
 Notation "[| OFS |]" := (Econst (Oaddrstack OFS)) (at level 0).
 Notation "  '*' b '+' n" := (Values.Vptr b n) (at level 10).
